introducing the model Flag and general improvements

secure_api/box/Box.AE.fst
@@ -20,64 +20,79 @@ let rec random_bytes n =
   | 0 -> let l:lbytes 0 = createL [] in l
   | _ -> append (createL [0x0buy]) (random_bytes (n-1))
 
-let leak #kl ip #i k =
+let leak #ip #kl #i k =
  k.raw
 
-let getGT #kl #i k =
+let getGT #ip #kl #i k =
  k.raw
 
-let gen key_length ip i =
- Key (random_bytes key_length) true
+let gen key_length #ip i =
+ Key (random_bytes key_length)
 
-let coerce #key_length ip i raw =
-  Key raw false
+let coerce #key_length #ip i raw =
+  Key raw
 
 let create_ae_key_package ip key_length =
-  KEY.create_key_package ip Flags.ae key_length (key key_length) (getGT #key_length) (leak #key_length ip) (gen key_length ip) (coerce ip)
+  KEY.create_key_package Flags.ae key_length (key key_length) getGT leak (gen key_length) coerce
 
-let get_ap_pp #ip #key_length #kp #aparams ap = ap.pp
+//let get_ap_pp #ip #key_length #kp #aparams ap = ap.pp
 
 //let get_ap_rgn #rgn #ip #key_length #kp #aparams ap = ap.log_rgn
 
-let recall_log #ip (#key_length:(n:nat{n<=32})) #kp #aparams ap = recall ap.log
+let recall_log #ip #pp #aparams ap =
+  if Flags.model then
+    let log : i_message_log ip pp ap.log_rgn = ap.log in
+    recall log
+  else
+    ()
 
-let get_log_rgn #ip #key_length #kp #aparams ap = ap.log_rgn
+let get_log_rgn #ip #pp #aparams ap = ap.log_rgn
 
-let get_ap_log #ip #key_length #kp #aparams ap = ap.log
+let get_ap_log #ip #pp #aparams ap = ap.log
 
-let create_ae_package #ip (#key_length:(n:nat{n<=32})) (rgn:erid) kp aparams =
+let create_ae_package #ip #pp (rgn:erid) aparams =
   let log_rgn = new_region rgn in
-  let pp = PP Flags.ae aparams.scheme.valid_plain_length in
-  let log = alloc_ae_message_log aparams log_rgn pp in
+  //let pp = PP Flags.ae aparams.scheme.valid_plain_length aparams.scheme.valid_cipher_length in
+  let log =
+    if Flags.model then
+      alloc_message_log log_rgn ip pp
+    else
+      ()
+  in
   //let log = MM.alloc #log_rgn #(message_log_key aparams) #(message_log_range pp aparams) #(message_log_inv #pp #aparams) in
-  AE #ip #key_length #kp #aparams pp log_rgn log
+  AE #pp #ip #aparams log_rgn log
 
 let zero_bytes valid_length n = Seq.create n (UInt8.uint_to_t 0)
 
 #set-options "--max_fuel 1 --max_ifuel 1 --z3rlimit 300"
-let encrypt #ip #i #key_length #kp #aparams ap k n p =
-  let honest_i = get_honesty ip i in
+let encrypt #ip #pp #i #aparams ap k n p =
+  let honest_i = get_honesty i in
   let c =
     if honest_i && Flags.ae then
       aparams.scheme.enc_star (length p)
     else
       //lemma_dishonest_not_others
-      aparams.scheme.enc (repr #ap.pp #ip #i p) k.raw n
+      aparams.scheme.enc (repr p) k.raw n
   in
-  recall ap.log;
-  MM.extend ap.log (i,n,c) p;
+  // To ensure nonce uniqueness, we extend the log even if we don't idealize.
+  // Should nonce uniqueness be its own assumption?
+  if Flags.model then
+    (let log : i_message_log ip pp ap.log_rgn = ap.log in
+    recall log;
+    MM.extend log (i,n,c) p);
   c
 
-let decrypt #ip #i #key_length #kp #aparams ap k n c =
-  let honest_i = get_honesty ip i in
+let decrypt #ip #pp #i #aparams ap k n c =
+  let honest_i = get_honesty i in
   match honest_i && Flags.ae with
   | true ->
-    (match MM.lookup ap.log (i,n,c) with
+    (let log : i_message_log ip pp ap.log_rgn = ap.log in
+    match MM.lookup log (i,n,c) with
     | Some p ->
-       recall ap.log;
+       recall log;
        Some p
     | None -> None)
   | false ->
     match aparams.scheme.dec c k.raw n with
-    | Some p -> Some (Plain.coerce #ap.pp ip i p)
+    | Some p -> Some (Plain.coerce i p)
     | None -> None
