secure_api/box/Box.AE.fsti
@@ -20,35 +20,31 @@ module MM = FStar.Monotonic.Map
 
 val random_bytes: n:(n:nat{n<=32}) -> lbytes n
 
-let bytes32 = b:bytes
-//let bytes32 = b:bytes{Seq.length b <= 32}
-
-noeq abstract type key (key_length:(n:nat{n<=32})) (i:inst_id) =
+noeq abstract type key (#ip:index_package) (key_length:(n:nat{n<=32})) (i:id ip) =
      | Key:
        raw: lbytes key_length ->
-       h:bool ->
-       key key_length i
+       key #ip key_length i
 
-val leak: #key_length:(n:nat{n<=32}) -> ip:index_package -> #i:inst_id{~Flags.ae \/ dishonest ip i} -> k:key key_length i -> raw:lbytes key_length{raw = k.raw}
+val leak: #key_length:(n:nat{n<=32}) -> #ip:index_package -> #i:id ip{~Flags.ae \/ corrupt i} -> k:key key_length i -> raw:lbytes key_length{raw = k.raw}
 
-val getGT: #key_length:(n:nat{n<=32}) -> #i:inst_id -> k:key key_length i -> GTot (raw:lbytes key_length{raw = k.raw})
+val getGT: #key_length:(n:nat{n<=32}) -> (#ip:index_package) -> #i:id ip -> k:key key_length i -> GTot (raw:lbytes key_length{raw = k.raw})
 
-val gen: key_length:(n:nat{n<=32}) -> ip:index_package -> i:inst_id -> k:key key_length i
+val gen: key_length:(n:nat{n<=32}) -> #ip:index_package -> i:id ip -> k:key key_length i
 
-val coerce: #key_length:(n:nat{n<=32}) -> ip:index_package -> i:inst_id{~Flags.ae \/ dishonest ip i} -> raw:lbytes key_length -> k:key key_length i{k.raw = raw}
+val coerce: #key_length:(n:nat{n<=32}) -> #ip:index_package -> i:id ip{~Flags.ae \/ corrupt i} -> raw:lbytes key_length -> k:key key_length i{k.raw = raw}
 
-val create_ae_key_package: ip:index_package -> key_length:(n:nat{n<=32}) -> KEY.key_package ip key_length (key key_length)
-
+val create_ae_key_package: ip:index_package -> key_length:(n:nat{n<=32}) -> KEY.key_package ip
 
 // Definition AE package
-noeq type encryption_scheme (key_length:(n:nat{n<=32})) (nonce_length:(n:nat{n<=32})) =
+
+let plain_package = pp:plain_package{pp.flag == Flags.ae}
+
+noeq type encryption_scheme (key_length:(n:nat{n<=32})) (pp:plain_package)=
   | ES:
-    valid_plain_length:(nat -> bool) ->
-    valid_cipher_length:(nat -> bool) ->
     gen: (unit -> lbytes key_length) ->
-    enc: (p:bytes32{valid_plain_length (Seq.length p)} -> k:lbytes key_length -> n:lbytes nonce_length -> c:bytes32{valid_cipher_length (Seq.length c)}) ->
-    enc_star: (plain_length:n32{valid_plain_length plain_length} -> c:bytes32{valid_cipher_length (Seq.length c)}) ->
-    dec: (c:bytes32{valid_cipher_length (Seq.length c)} -> k:lbytes key_length -> n:lbytes nonce_length -> option (p:bytes32{valid_plain_length (Seq.length p)})) ->
+    enc: (p:plain pp -> k:lbytes key_length -> n:nonce pp -> c:cipher pp) ->
+    enc_star: (plain_length:nat{pp.valid_plain_length plain_length} -> c:cipher pp) ->
+    dec: (c:cipher pp -> k:lbytes key_length -> n:nonce pp -> option (p:plain pp)) ->
 //    correctness: (p:bytes -> k:lbytes key_length -> n:lbytes nonce_length -> Lemma
 //    (requires True)
 //    (ensures (
@@ -57,143 +53,122 @@ noeq type encryption_scheme (key_length:(n:nat{n<=32})) (nonce_length:(n:nat{n<=
 //      /\ Some?.v dec_result == p
 //    ))
       //    ) ->
-    encryption_scheme key_length nonce_length
+    encryption_scheme key_length pp
 
 // Make them abstract or move the flag to ae_package?
-noeq type ae_parameters =
+noeq type ae_parameters (pp:plain_package) =
   | GP:
     keylength:(n:nat{n<=32}) ->
-    nonce_length:(n:nat{n<=32}) ->
-    scheme: (encryption_scheme keylength nonce_length) ->
-    ae_parameters
+    scheme: (encryption_scheme keylength pp) ->
+    ae_parameters pp
 
-//let nonce (#key_length:(n:nat{n<=32})) (#kp:KEY.key_package #key_length key) (#pp:plain_package) (ap:ae_parameters kp pp) = lbytes ap.nonce_length
-let nonce (aparams:ae_parameters) = lbytes aparams.nonce_length
-let ciphertext (aparams:ae_parameters) = c:bytes32{aparams.scheme.valid_cipher_length (Seq.length c)}
-
-let fst t = Mktuple3?._1 t
-let snd t = Mktuple3?._2 t
-let thrd t = Mktuple3?._3 t
-
-//type message_log_key (aparams:ae_parameters) = inst_id*nonce aparams*ciphertext aparams
-////  | LOG_KEY: i:inst_id -> n:nonce aparams -> c:ciphertext aparams -> message_log_key aparams
-//
-//let message_log_value (pp:plain_package) (i:inst_id) = protected_plain pp i
-//let message_log_range (pp:plain_package) (aparams:ae_parameters) (k:message_log_key aparams) = message_log_value pp (Mktuple3?._1 k)
-//let message_log_inv (#pp:plain_package) (#aparams:ae_parameters) (f:MM.map' (message_log_key aparams) (message_log_range pp aparams)) = True
-//
-//let message_log (#pp:plain_package) (rgn:erid) (aparams:ae_parameters) =
-//  MM.t rgn (message_log_key aparams) (message_log_range pp aparams) (message_log_inv)
-//
-//let empty_message_log (aparams:ae_parameters) (pp:plain_package) = MM.empty_map (message_log_key aparams) (message_log_range pp aparams)
-
-let ae_message_log (aparams:ae_parameters) = Mem.message_log (nonce aparams) (ciphertext aparams)
-let empty_ae_message_log (aparams:ae_parameters) = Mem.empty_message_log (nonce aparams) (ciphertext aparams)
-let alloc_ae_message_log (aparams:ae_parameters) = Mem.alloc_message_log (nonce aparams) (ciphertext aparams)
-
-noeq abstract type ae_package (#ip:index_package) (#key_length:(n:nat{n<=32})) (kp:KEY.key_package ip key_length (key key_length)) (aparams:ae_parameters{aparams.keylength = key_length}) =
+noeq abstract type ae_package (#pp:plain_package) (ip:index_package) (aparams:ae_parameters pp) =
   | AE:
-    pp:plain_package{pp == PP Flags.ae aparams.scheme.valid_plain_length} ->
     log_rgn:erid ->
-    log:ae_message_log aparams pp log_rgn ->
-    ae_package #ip #key_length kp aparams
+    log:message_log ip pp log_rgn ->
+    ae_package #pp ip aparams
 
-//val get_flag: (#ip:index_package rgn) -> (#key_length:(n:nat{n<=32})) -> (#kp:KEY.key_package ip key_length (key key_length)) -> (#aparams:ae_parameters{aparams.keylength = key_length}) -> ap:ae_package kp aparams -> GTot (b:bool{b = ap.b})
-//let valid_ae_plain_package (aparams:ae_parameters) (pp:plain_package) = pp == PP (get_ae_flagGT aparams) aparams.scheme.valid_plain_length
-
-val get_ap_pp: (#ip:index_package) -> (#key_length:(n:nat{n<=32})) -> (#kp:KEY.key_package ip key_length (key key_length)) -> (#aparams:ae_parameters{aparams.keylength = key_length}) -> (ap:ae_package #ip #key_length kp aparams) -> pp:plain_package{pp.flag == Flags.ae /\ pp.valid_length == aparams.scheme.valid_plain_length /\ pp == ap.pp}
-
-//val get_ap_rgn: (#ip:index_package rgn) -> (#key_length:(n:nat{n<=32})) -> (#kp:KEY.key_package ip key_length (key key_length)) -> (#aparams:ae_parameters{aparams.keylength = key_length}) -> (ap:ae_package #rgn #ip #key_length kp aparams) -> rgn:erid{rgn = ap.rgn}
-
-val recall_log: (#ip:index_package) -> (#key_length:(n:nat{n<=32})) -> (#kp:KEY.key_package ip key_length (key key_length)) -> (#aparams:ae_parameters{aparams.keylength = key_length}) -> (ap:ae_package kp aparams) -> ST unit
+val recall_log: (#ip:index_package) -> (#pp:plain_package) -> (#aparams:ae_parameters pp) -> (ap:ae_package ip aparams) -> ST unit
   (requires (fun h0 -> True))
   (ensures (fun h0 _ h1 ->
     h0 == h1
-    /\ contains h1 ap.log
+    /\ (Flags.model ==>
+      (let log : i_message_log ip pp ap.log_rgn = ap.log in
+      contains h1 log))
   ))
 
-val get_log_rgn: (#ip:index_package) -> (#key_length:(n:nat{n<=32})) -> (#kp:KEY.key_package ip key_length (key key_length)) -> (#aparams:ae_parameters{aparams.keylength = key_length}) -> (ap:ae_package kp aparams) -> Tot (rgn:erid{rgn = ap.log_rgn})
+val get_log_rgn: (#ip:index_package) -> (#pp:plain_package) -> (#aparams:ae_parameters pp) -> (ap:ae_package ip aparams) -> Tot (rgn:erid{rgn = ap.log_rgn})
 
-val get_ap_log: (#ip:index_package) -> (#key_length:(n:nat{n<=32})) -> (#kp:KEY.key_package ip key_length (key key_length)) -> (#aparams:ae_parameters{aparams.keylength = key_length}) -> (ap:ae_package kp aparams) -> GTot (ae_message_log  aparams (get_ap_pp ap) (get_log_rgn ap))
+val get_ap_log: (#ip:index_package) -> (#pp:plain_package) -> (#aparams:ae_parameters pp) -> (ap:ae_package ip aparams) -> GTot (message_log ip pp (get_log_rgn ap))
 
-let nonce_is_unique (#ip:index_package) (#key_length:(n:nat{n<=32})) (#kp:KEY.key_package ip key_length (key key_length)) (#aparams:ae_parameters{aparams.keylength = key_length}) (ap:ae_package kp aparams) (i:inst_id) (n:nonce aparams) (h0:mem) =
-  forall c . MM.fresh ap.log (i,n,c) h0
+let nonce_is_unique (#ip:index_package) (#pp:plain_package)  (#aparams:ae_parameters pp) (ap:ae_package ip aparams) (i:id ip) (n:nonce pp) (h0:mem) =
+  Flags.model ==> (
+    let log : i_message_log ip pp ap.log_rgn = ap.log in
+    forall c . MM.fresh log (i,n,c) h0)
 
-val create_ae_package: (#ip:index_package) -> (#key_length:(n:nat{n<=32})) -> (rgn:erid) -> (kp:KEY.key_package ip key_length (key key_length)) -> (aparams:ae_parameters{aparams.keylength = key_length}) -> ST (ae_package kp aparams)
+val create_ae_package: (#ip:index_package) -> (#pp:plain_package) -> (rgn:erid) -> (aparams:ae_parameters pp) -> ST (ae_package ip aparams)
   (requires (fun h0 -> True))
   (ensures (fun h0 ap h1 ->
-    modifies (Set.singleton rgn) h0 h1
-    /\ (forall n i . nonce_is_unique ap i n h1)
-    /\ extends ap.log_rgn rgn
-    /\ contains h1 ap.log
-    /\ sel h1 ap.log == empty_ae_message_log aparams ap.pp
+    if Flags.model then
+      let log : i_message_log ip pp ap.log_rgn = ap.log in
+      modifies (Set.singleton rgn) h0 h1
+      /\ (forall n i . nonce_is_unique ap i n h1)
+      /\ extends ap.log_rgn rgn
+      /\ sel h1 log == empty_message_log ip pp
+      /\ contains h1 log
+    else
+      modifies_none h0 h1
   ))
 
-val zero_bytes: (valid_length:(n:n32 -> bool)) -> (n:n32{valid_length n}) -> p:lbytes n{valid_length (Seq.length p)}
+val zero_bytes: (valid_length:(n:nat -> bool)) -> (n:nat{valid_length n}) -> p:lbytes n{valid_length (Seq.length p)}
 
-let encrypt_modified_regions (#ip:index_package) (#key_length:(n:nat{n<=32})) (#kp:KEY.key_package ip key_length (key key_length)) (#aparams:ae_parameters{aparams.keylength = key_length}) (ap:ae_package kp aparams) : (Set.set rid) = Set.singleton ap.log_rgn
+let encrypt_footprint (#ip:index_package) (#pp:plain_package) (#aparams:ae_parameters pp) (ap:ae_package ip aparams) (h0:mem) (h1:mem) =
+  if Flags.model then
+    modifies (Set.singleton ap.log_rgn) h0 h1
+  else
+    h0 == h1
 
-let encrypt_log_change (#ip:index_package) (#key_length:(n:nat{n<=32})) (#kp:KEY.key_package ip key_length (key key_length)) (#aparams:ae_parameters{aparams.keylength = key_length}) (ap:ae_package kp aparams) (i:inst_id) (n:nonce aparams) (c:ciphertext aparams) (p:protected_plain ap.pp i) (h0:mem) (h1:mem) =
-    let a = 1 in
-    witnessed (MM.contains ap.log (i,n,c) p)
-    /\ contains h0 ap.log
-    /\ sel h1 ap.log == MM.upd (sel h0 ap.log) (i,n,c) p
+let encrypt_log_change (#ip:index_package) (#pp:plain_package) (#aparams:ae_parameters pp) (ap:ae_package ip aparams) (i:id ip) (n:nonce pp) (c:cipher pp) (p:protected_plain pp i) (h0:mem) (h1:mem) =
+  Flags.model ==>
+    (let log : i_message_log ip pp ap.log_rgn = ap.log in
+    witnessed (MM.contains log (i,n,c) p)
+    /\ contains h0 log
+    /\ sel h1 log == MM.upd (sel h0 log) (i,n,c) p)
 
-let encrypt_functional_spec (#ip:index_package) (#i:inst_id) (#key_length:(n:nat{n<=32})) (#kp:KEY.key_package ip key_length (key key_length)) (#aparams:ae_parameters{aparams.keylength = key_length}) (ap:ae_package kp aparams) (k:key key_length i) (n:nonce aparams) (c:ciphertext aparams) (p:protected_plain ap.pp i) =
-  let a = 1 in
-  ((honest ip i /\ Flags.ae) ==>
+let encrypt_functional_spec (#ip:index_package) (#pp:plain_package) (#i:id ip) (#aparams:ae_parameters pp) (ap:ae_package ip aparams) (k:key aparams.keylength i) (n:nonce pp) (c:cipher pp) (p:protected_plain pp i) =
+  ((honest i /\ Flags.ae) ==>
     (c = aparams.scheme.enc_star (length p)))
-  /\ ((dishonest ip i \/ ~Flags.ae) ==>
-    (c = aparams.scheme.enc (repr #ap.pp #ip #i p) k.raw n))
+  /\ ((corrupt i \/ ~Flags.ae) ==>
+    (c = aparams.scheme.enc (repr p) k.raw n))
 
 #set-options "--max_fuel 1 --max_ifuel 1 --z3rlimit 300"
-val encrypt: #ip:index_package -> #i:inst_id -> #key_length:(n:nat{n<=32}) -> #kp:KEY.key_package ip key_length (key key_length) -> #aparams:ae_parameters{key_length = aparams.keylength} -> ap:ae_package kp aparams -> k:key key_length i -> n:nonce aparams -> p:protected_plain ap.pp i -> ST (ciphertext aparams)
+val encrypt: #ip:index_package -> #pp:plain_package -> #i:id ip -> #aparams:ae_parameters pp -> ap:ae_package ip aparams -> k:key aparams.keylength i -> n:nonce pp -> p:protected_plain pp i -> ST (cipher pp)
   (requires (fun h0 ->
     (nonce_is_unique ap i n h0)
-    /\ registered ip i
+    /\ registered i
   ))
   (ensures (fun h0 c h1 ->
     encrypt_functional_spec ap k n c p
     /\ encrypt_log_change ap i n c p h0 h1
-    /\ modifies (encrypt_modified_regions ap) h0 h1
+    /\ encrypt_footprint ap h0 h1
     /\ ((forall n'. nonce_is_unique ap i n' h0) ==> (forall n' . n' =!=n ==> nonce_is_unique ap i n' h1))
   ))
 
-let decrypt_modified_regions (#ip:index_package) (#key_length:(n:nat{n<=32})) (#kp:KEY.key_package ip key_length (key key_length)) (#aparams:ae_parameters{aparams.keylength = key_length}) (ap:ae_package kp aparams) = Set.empty
+let decrypt_footprint (#ip:index_package) (#pp:plain_package) (#aparams:ae_parameters pp) (ap:ae_package ip aparams) (h0:mem) (h1:mem) = h0 == h1
 
-let decrypt_log_change (#ip:index_package) (#key_length:(n:nat{n<=32})) (#kp:KEY.key_package ip key_length (key key_length)) (#aparams:ae_parameters{aparams.keylength = key_length}) (ap:ae_package kp aparams) (h0:mem) (h1:mem) =
-  sel h1 ap.log == sel h0 ap.log
+let decrypt_log_change (#ip:index_package) (#pp:plain_package) (#aparams:ae_parameters pp) (ap:ae_package ip aparams) (h0:mem) (h1:mem) =
+  Flags.model ==>
+    (let log : i_message_log ip pp ap.log_rgn = ap.log in
+    sel h1 log == sel h0 log)
 
-
-let decrypt_functional_spec (#ip:index_package)
-                            (#i:inst_id)
-                            (#key_length:(n:nat{n<=32}))
-                            (#kp:KEY.key_package ip key_length (key key_length))
-                            (#aparams:ae_parameters{aparams.keylength = key_length})
-                            (ap:ae_package kp aparams)
-                            (k:key key_length i)
-                            (n:nonce aparams)
-                            (c:ciphertext aparams)
-                            (p:option (protected_plain ap.pp i))
+let decrypt_functional_spec (#pp:plain_package)
+                            (#ip:index_package)
+                            (#i:id ip)
+                            (#aparams:ae_parameters pp)
+                            (ap:ae_package ip aparams)
+                            (k:key aparams.keylength i)
+                            (n:nonce pp)
+                            (c:cipher pp)
+                            (p:option (protected_plain pp i))
                             (h0:mem) =
-  let a = 1 in
-    ((honest ip i /\ Flags.ae) ==>
-      (match p with
-       | Some p' -> MM.contains ap.log (i,n,c) p' h0
-       | None -> MM.fresh ap.log (i,n,c) h0
+    ((honest i /\ Flags.ae) ==>
+      (let log : i_message_log ip pp ap.log_rgn = ap.log in
+      match p with
+       | Some p' -> MM.contains log (i,n,c) p' h0
+       | None -> MM.fresh log (i,n,c) h0
       ))
-    /\ ((dishonest ip i \/ ~Flags.ae) ==>
+    /\ ((corrupt i \/ ~Flags.ae) ==>
       (match aparams.scheme.dec c k.raw n with
-       | Some p' -> Some? p /\ Some?.v p == Plain.coerce ip i p'
+       | Some p' -> Some? p /\ Some?.v p == Plain.coerce i p'
        | None -> None? p
       ))
 
-val decrypt: #ip:index_package -> #i:inst_id -> #key_length:(n:nat{n<=32}) -> #kp:KEY.key_package ip key_length (key key_length) -> #aparams:ae_parameters{key_length = aparams.keylength} -> ap:ae_package kp aparams -> k:key key_length i -> n:nonce aparams -> c:ciphertext aparams -> ST (option (p:protected_plain ap.pp i))
+val decrypt: #ip:index_package -> #pp:plain_package -> #i:id ip -> #aparams:ae_parameters pp -> ap:ae_package ip aparams -> k:key aparams.keylength i -> n:nonce pp -> c:cipher pp -> ST (option (p:protected_plain pp i))
   (requires (fun h0 ->
-    registered ip i
+    registered i
   ))
   (ensures (fun h0 p h1 ->
     decrypt_functional_spec ap k n c p h0
-    /\ modifies (decrypt_modified_regions ap) h0 h1
+    /\ decrypt_footprint ap h0 h1
     /\ decrypt_log_change ap h0 h1
   ))
