secure_api/box/Box.Key.fst
@@ -7,33 +7,27 @@ open FStar.Endianness
 open Box.Index
 
 // Definition KEY package
-noeq type key_package (ip:index_package) (key_length:(n:nat{n<=32})) (key_type:(inst_id  -> Type0)) =
+noeq type key_package (ip:index_package) =
   | KP:
   flag: Type0 ->
-  getGT: (#i:inst_id -> k:key_type i -> GTot (lbytes key_length)) ->
-  leak: (#i:inst_id{dishonest ip i \/ ~flag} -> k:key_type i -> (raw:lbytes key_length{raw = getGT k})) ->
-  gen: (i:inst_id -> k:key_type i) ->
-  coerce: (i:inst_id{~flag \/ dishonest ip i} -> raw:lbytes key_length -> (k:key_type i{raw = getGT k})) ->
-  key_package ip key_length key_type
+  key_length:(n:nat{n<=32}) ->
+  key_type:(id ip  -> Type0) ->
+  getGT: (#i:id ip -> k:key_type i -> GTot (lbytes key_length)) ->
+  leak: (#i:id ip{corrupt i \/ ~flag} -> k:key_type i -> (raw:lbytes key_length{raw = getGT k})) ->
+  gen: (i:id ip -> k:key_type i) ->
+  coerce: (i:id ip{~flag \/ corrupt i} -> raw:lbytes key_length -> (k:key_type i{raw = getGT k})) ->
+  key_package ip
 
 #set-options "--z3rlimit 300 --max_ifuel 1 --max_fuel 0"
 val create_key_package:
-  (ip:index_package) ->
+  (#ip:index_package) ->
   (flag:Type0) ->
   (key_length:(n:nat{n<=32})) ->
-  (key_type:(inst_id -> Type0)) ->
-  (param_getGT: (#i:inst_id -> k:key_type i -> GTot (lbytes key_length))) ->
-  (param_leak: (#i:inst_id{dishonest ip i \/ ~flag} -> k:key_type i -> (raw:lbytes key_length{raw = param_getGT k}))) ->
-  (param_gen: (i:inst_id -> k:key_type i)) ->
-  (param_coerce: (i:inst_id{dishonest ip i \/ ~flag} -> raw:lbytes key_length -> (k:key_type i{raw = param_getGT k}))) ->
-  (kp:key_package ip key_length key_type{True
-//    param_hon == hon kp
-//    /\ param_hon == kp.hon
-//    /\ param_getGT == kp.getGT
-//    /\ param_getGT == getGT kp
-//    /\ param_cget == cget kp
-//    /\ param_gen == gen kp
-//    /\ param_cset == cset kp
-  })
-let create_key_package ip flag key_length key_type getGT leak gen coerce =
-  KP flag getGT leak gen coerce
+  (key_type:(id ip -> Type0)) ->
+  (param_getGT: (#i:id ip -> k:key_type i -> GTot (lbytes key_length))) ->
+  (param_leak: (#i:id ip{corrupt i \/ ~flag} -> k:key_type i -> (raw:lbytes key_length{raw = param_getGT k}))) ->
+  (param_gen: (i:id ip -> k:key_type i)) ->
+  (param_coerce: (i:id ip{corrupt i \/ ~flag} -> raw:lbytes key_length -> (k:key_type i{raw = param_getGT k}))) ->
+  (kp:key_package ip)
+let create_key_package #ip flag key_length key_type getGT leak gen coerce =
+  KP flag key_length key_type getGT leak gen coerce
