secure_api/box/Box.ODH.fst
@@ -22,59 +22,72 @@ let get_share_raw #oparams sh = sh.raw_sh
 
 let get_exponent_raw #oparams exp = exp.raw_exp
 
-let gen_dh_footprint ip oparams h0 h1 =
+let create_odh_index_package rgn oparams =
+  create_leaf_index_package rgn (lbytes oparams.share_length)
+
+let gen_dh_footprint oparams ip h0 h1 =
   register_footprint ip h0 h1
 
-let gen_dh ip oparam =
-  let raw_exp = random_bytes oparam.exponent_length in
-  let raw_sh = oparam.exponentiate raw_exp oparam.generator in
+#set-options "--z3rlimit 50 --max_ifuel 2 --max_fuel 2 --print_implicits"
+let gen_dh oparams ip =
+  let raw_exp = random_bytes oparams.exponent_length in
+  let raw_sh = oparams.exponentiate raw_exp oparams.generator in
   let h0 = get() in
-  assume(fresh ip (PK_id raw_sh) h0);
-  register ip (PK_id raw_sh) true;
+  assume(fresh #ip raw_sh h0); // Fixme!
+  register #ip raw_sh true;
   let sh = SH raw_sh in
-  (EXP raw_exp sh,sh)
+  let exp = EXP raw_exp sh in
+  exp,sh
 
-let coerce_dh_sh_footprint ip oparams raw_sh h0 h1 =
+let coerce_dh_sh_footprint oparams ip raw_sh h0 h1 =
   register_footprint ip h0 h1
 
-let coerce_dh_sh ip oparam raw_sh =
-  register ip (PK_id raw_sh) false;
+let coerce_dh_sh oparam ip raw_sh =
   SH raw_sh
 
-let coerce_dh_exp_footprint ip oparams raw_sh h0 h1 =
+let coerce_dh_exp_footprint oparams ip raw_sh h0 h1 =
   register_footprint ip h0 h1
 
-let coerce_dh_exp ip oparam raw_exp =
+let coerce_dh_exp oparam ip raw_exp =
   let raw_sh = oparam.exponentiate raw_exp oparam.generator in
-  register ip (PK_id raw_sh) false;
   let sh = SH raw_sh in
   EXP raw_exp sh
 
-let get_op_rgn #ip #key_length #key_type #kp #oparam op = op.kp_log_rgn
+let get_op_rgn #oparams #ip #kp op = op.log_rgn
 
-let get_op_log #ip #key_length #key_type #kp #oparam op = op.kp_log
+let get_op_log #oparams #ip #kp op = op.log
 
-let recall_op_log #ip #key_length #key_type #kp #oparam op =
-  recall op.kp_log
+let recall_op_log #oparams #ip #kp op =
+  if Flags.model then
+    let log:i_key_log op.log_rgn (composed_ip ip) kp.key_type = op.log in
+    recall log
+  else
+    ()
 
-let create_odh_package #ip #key_length #key_type rgn kp oparam =
+let create_odh_package #oparams ip rgn kp =
   let odh_rgn = new_region rgn in
-  let kp_log = MM.alloc #odh_rgn #key_package_log_key #(key_package_log_range key_type) #(key_package_log_inv key_type) in
+  let kp_log =
+    if Flags.model then
+      MM.alloc #odh_rgn #(key_log_key (composed_ip ip)) #(key_log_range (composed_ip ip) kp.key_type) #(key_log_inv (composed_ip ip) kp.key_type)
+    else
+      ()
+  in
   ODH odh_rgn kp_log
 
-#set-options "--z3rlimit 300 --max_ifuel 2 --max_fuel 1"
-let dh_op #ip #key_length #key_type #kp #oparam op sh exp =
-  let i = compose_id (PK_id sh.raw_sh) (PK_id exp.sh.raw_sh) in
-  let both_honest = get_honesty ip i in
+#set-options "--z3rlimit 300 --max_ifuel 2 --max_fuel 2"
+let dh_op #oparams #ip #kp op sh exp =
+  let h0 = get() in
+  let i:id (composed_ip ip) = composed_id sh exp.sh in
+  let both_honest = get_honesty #(composed_ip ip) i in
     if Flags.prf_odh && both_honest then
-      (recall op.kp_log;
-      match MM.lookup op.kp_log i with
+      let log:i_key_log op.log_rgn (composed_ip ip) kp.key_type = op.log in
+      (recall log;
+      match MM.lookup log i with
       | None ->
-        //let k:(k:key_type i{kp.hon k = true}) = kp.gen i in
         let k = kp.gen i in
-        MM.extend op.kp_log i k;
+        MM.extend log i k;
         k
       | Some k -> k)
     else
-      (recall op.kp_log;
-      kp.coerce i (oparam.hash (oparam.exponentiate exp.raw_exp sh.raw_sh)))
+      (recall_op_log op;
+      kp.coerce i (oparams.hash (oparams.exponentiate exp.raw_exp sh.raw_sh)))
