secure_api/box/Box.ODH.fsti
@@ -12,19 +12,15 @@ open FStar.Endianness
 
 module MM = FStar.Monotonic.Map
 
-val random_bytes: n:nat{n<=32} -> lbytes n
+let n32 = n:nat{n<=32}
 
-//val random_bytes: n:nat{n<=32} -> ST (lbytes n)
-//  (requires (fun h0 -> True))
-//  (ensures (fun h0 b h1 ->
-//    h0 == h1
-//  ))
+val random_bytes: n:n32 -> lbytes n
 
 noeq type odh_parameters =
   | OP:
-  share_length:(n:nat{n=32}) ->
-  exponent_length:(n:nat{n=32}) ->
-  hash_length:(n:nat{n=32}) ->
+  share_length:(n:n32) ->
+  exponent_length:(n:n32) ->
+  hash_length:(n:n32) ->
   generator:lbytes share_length ->
   exponentiate:(lbytes exponent_length -> lbytes share_length -> lbytes share_length) ->
   hash:(lbytes share_length -> lbytes hash_length) ->
@@ -47,132 +43,215 @@ val get_share_raw: #oparams:odh_parameters -> sh:share oparams -> raw:lbytes opa
 
 val get_exponent_raw: #oparams:odh_parameters -> exp:exponent oparams -> GTot (raw:lbytes oparams.exponent_length{raw = exp.raw_exp})
 
-val gen_dh_footprint: ip:index_package -> oparam:odh_parameters -> h0:mem -> h1:mem -> Type0
+let odh_index_package (oparams:odh_parameters) = ip:index_package{
+  Leaf_IP? ip
+  /\ (match ip with
+    | Leaf_IP t rgn log -> t == lbytes oparams.share_length)
+  }
 
-val gen_dh: (ip:index_package) -> (oparam:odh_parameters) -> ST (dh_keypair:(exponent oparam*share oparam))
+val create_odh_index_package: rgn:erid -> oparams:odh_parameters -> ST (odh_index_package oparams)
   (requires (fun h0 -> True))
-  (ensures (fun h0 (e,sh) h1 ->
+  (ensures (fun h0 ip h1 ->
+    create_leaf_index_package_footprint rgn (lbytes oparams.share_length) ip h0 h1
+  ))
+
+val gen_dh_footprint: oparams:odh_parameters -> ip:odh_index_package oparams -> h0:mem -> h1:mem -> Type0
+
+val gen_dh: (oparams:odh_parameters) -> (ip:odh_index_package oparams) -> ST (dh_keypair:(exponent oparams*share oparams))
+  (requires (fun h0 ->
+    Flags.model))
+  (ensures (fun h0 dh_pair h1 ->
+    let e,sh = dh_pair in
+    let i:id ip = sh.raw_sh in
     e.sh == sh
-    /\ registered ip (PK_id sh.raw_sh)
-    /\ honest ip (PK_id sh.raw_sh)
-    /\ gen_dh_footprint ip oparam h0 h1
+    /\ registered i
+    /\ honest i
+    /\ gen_dh_footprint oparams ip h0 h1
   ))
 
-val coerce_dh_sh_footprint: (ip:index_package) -> (oparam:odh_parameters) -> (raw_sh:lbytes oparam.share_length) -> h0:mem -> h1:mem -> Type0
+val coerce_dh_sh_footprint: (oparams:odh_parameters) -> (ip:odh_index_package oparams) -> (raw_sh:lbytes oparams.share_length) -> h0:mem -> h1:mem -> Type0
 
-val coerce_dh_sh: (ip:index_package) -> (oparam:odh_parameters) -> (raw_sh:lbytes oparam.share_length) -> ST (sh:share oparam{sh.raw_sh = raw_sh})
+val coerce_dh_sh: (oparams:odh_parameters) -> (ip:odh_index_package oparams) -> (raw_sh:lbytes oparams.share_length) -> ST (sh:share oparams{sh.raw_sh = raw_sh})
   (requires (fun h0 ->
-    fresh ip (PK_id raw_sh) h0
+    registered #ip raw_sh
+    /\ corrupt #ip raw_sh
   ))
   (ensures (fun h0 sh h1 ->
-    registered ip (PK_id raw_sh)
-    /\ dishonest ip (PK_id raw_sh)
-    /\ coerce_dh_sh_footprint ip oparam raw_sh h0 h1
+    coerce_dh_sh_footprint oparams ip raw_sh h0 h1
   ))
 
-val coerce_dh_exp_footprint: (ip:index_package) -> (oparam:odh_parameters) -> (raw_exp:lbytes oparam.exponent_length) -> h0:mem -> h1:mem -> Type0
+val coerce_dh_exp_footprint: (oparams:odh_parameters) -> (ip:odh_index_package oparams) -> (raw_exp:lbytes oparams.exponent_length) -> h0:mem -> h1:mem -> Type0
 
-val coerce_dh_exp: (ip:index_package) -> (oparam:odh_parameters) -> (raw_exp:lbytes oparam.exponent_length) -> ST (exp:exponent oparam{exp.raw_exp = raw_exp})
+val coerce_dh_exp: (oparams:odh_parameters) -> (ip:odh_index_package oparams) -> (raw_exp:lbytes oparams.exponent_length) -> ST (exp:exponent oparams{exp.raw_exp = raw_exp})
   (requires (fun h0 ->
-    let raw_sh = oparam.exponentiate raw_exp oparam.generator in
-    fresh ip (PK_id raw_sh) h0
+    let raw_sh = oparams.exponentiate raw_exp oparams.generator in
+    registered #ip raw_sh
+    /\ corrupt #ip raw_sh
   ))
   (ensures (fun h0 sh h1 ->
-    let raw_sh = oparam.exponentiate raw_exp oparam.generator in
-    registered ip (PK_id raw_sh)
-    /\ dishonest ip (PK_id raw_sh)
-    /\ coerce_dh_exp_footprint ip oparam raw_exp h0 h1
+    let raw_sh = oparams.exponentiate raw_exp oparams.generator in
+    coerce_dh_exp_footprint oparams ip raw_exp h0 h1
   ))
 
-let key_package_log_key = inst_id
-let key_package_log_value (i:inst_id) (key_type:(inst_id -> Type0)) = key_type i
-let key_package_log_range  (key_type:(inst_id -> Type0)) (k:key_package_log_key) = key_package_log_value k key_type
-let key_package_log_inv (key_type:(inst_id -> Type0)) (f:MM.map' (key_package_log_key) (key_package_log_range key_type)) = True
+let key_log_key (ip:index_package) = id ip
+let key_log_value (ip:index_package) (i:id ip) (key_type:(id ip -> Type0)) = key_type i
+let key_log_range (ip:index_package) (key_type:(id ip -> Type0)) (k:key_log_key ip) = key_log_value ip k key_type
+let key_log_inv (ip:index_package) (key_type:(id ip -> Type0)) (f:MM.map' (key_log_key ip) (key_log_range ip key_type)) = True
 
-let key_package_log (rgn:erid) (key_type:(inst_id -> Type0)) =
-  MM.t rgn (key_package_log_key) (key_package_log_range key_type) (key_package_log_inv key_type)
+let i_key_log (rgn:erid) (ip:index_package) (key_type:(id ip -> Type0)) =
+    MM.t rgn (key_log_key ip) (key_log_range ip key_type) (key_log_inv ip key_type)
 
-noeq abstract type odh_package (#ip:index_package) (#key_length:(n:nat{n<=32})) (#key_type:(inst_id -> Type0)) (kp:key_package ip key_length key_type) (oparam:odh_parameters{oparam.hash_length = key_length}) =
+let key_log (rgn:erid) (ip:index_package) (key_type:(id ip -> Type0)) =
+  if Flags.model then
+    i_key_log rgn ip key_type
+  else
+    unit
+
+let empty_key_log (ip:index_package) (key_type:(id ip -> Type0)) = MM.empty_map (key_log_key ip) (key_log_range ip key_type)
+
+let composed_ip (ip:index_package) = Node_IP [ip;ip]
+
+let key_package (ip:index_package) (oparams:odh_parameters) = kp:key_package ip {kp.key_length = oparams.hash_length}
+
+noeq abstract type odh_package (#oparams:odh_parameters) (ip:odh_index_package oparams) (kp:key_package (composed_ip ip) oparams) =
   | ODH:
-  kp_log_rgn:erid ->
-  kp_log:key_package_log kp_log_rgn key_type ->
-  odh_package #ip #key_length #key_type kp oparam
+  log_rgn:erid ->
+  log:key_log log_rgn (composed_ip ip) kp.key_type ->
+  odh_package #oparams ip kp
 
-val get_op_rgn: (#ip:index_package) -> (#key_length:(n:nat{n<=32})) -> (#key_type:(inst_id -> Type0)) -> (#kp:key_package ip key_length key_type) -> (#oparam:odh_parameters{oparam.hash_length = key_length}) -> op:odh_package kp oparam -> (rgn:erid{rgn = op.kp_log_rgn})
+val get_op_rgn: (#oparams:odh_parameters) -> (#ip:odh_index_package oparams) -> (#kp:key_package (composed_ip ip) oparams) -> op:odh_package ip kp -> (rgn:erid{rgn = op.log_rgn})
 
-val get_op_log: (#ip:index_package) -> (#key_length:(n:nat{n<=32})) -> (#key_type:(inst_id -> Type0)) -> (#kp:key_package ip key_length key_type) -> (#oparam:odh_parameters{oparam.hash_length = key_length}) -> op:odh_package kp oparam -> GTot (log:key_package_log op.kp_log_rgn key_type)
+val get_op_log: (#oparams:odh_parameters) -> (#ip:odh_index_package oparams) -> (#kp:key_package (composed_ip ip) oparams) -> op:odh_package ip kp -> GTot (log:key_log op.log_rgn (composed_ip ip) kp.key_type)
 
-val recall_op_log: (#ip:index_package) -> (#key_length:(n:nat{n<=32})) -> (#key_type:(inst_id -> Type0)) -> (#kp:key_package ip key_length key_type) -> (#oparam:odh_parameters{oparam.hash_length = key_length}) -> op:odh_package kp oparam -> ST unit
+val recall_op_log: (#oparams:odh_parameters) -> (#ip:odh_index_package oparams) -> (#kp:key_package (composed_ip ip) oparams) -> op:odh_package ip kp -> ST unit
   (requires (fun h0 -> True))
   (ensures (fun h0 _ h1 ->
-    h0 == h1
-    /\ contains h1 op.kp_log
+    (Flags.model ==>
+      (let log:i_key_log op.log_rgn (composed_ip ip) kp.key_type = op.log in
+      contains h1 log))
+    /\ h0 == h1
   ))
 
-val create_odh_package: (#ip:index_package) -> (#key_length:(n:nat{n<=32})) -> (#key_type:(inst_id -> Type0)) -> (rgn:erid) -> (kp:key_package ip key_length key_type) -> (oparam:odh_parameters{oparam.hash_length = key_length}) -> ST (odh_package #ip #key_length #key_type kp oparam)
+val create_odh_package: (#oparams:odh_parameters) -> (ip:odh_index_package oparams) -> (rgn:erid) -> (kp:key_package (composed_ip ip) oparams) -> ST (odh_package #oparams ip kp)
   (requires (fun h0 -> True))
   (ensures (fun h0 op h1 ->
-    modifies (Set.singleton op.kp_log_rgn) h0 h1
-    /\ extends op.kp_log_rgn rgn
+    if Flags.model then
+      let log:i_key_log op.log_rgn (composed_ip ip) kp.key_type = op.log in
+      modifies (Set.singleton op.log_rgn) h0 h1
+      /\ extends op.log_rgn rgn
+      /\ sel h1 log == empty_key_log (composed_ip ip) kp.key_type
+      /\ contains h1 log
+    else
+      modifies_none h0 h1
   ))
 
-let dh_op_memory_footprint (#ip:index_package) (#key_length:(n:nat{n<=32})) (#key_type:(inst_id -> Type0)) (#kp:key_package ip key_length key_type) (#oparam:odh_parameters{oparam.hash_length = key_length}) (op:odh_package kp oparam) (sh:share oparam) (exp:exponent oparam{exp.sh.raw_sh <> sh.raw_sh}) (h0:mem) (h1:mem) =
-  let i = compose_id (PK_id sh.raw_sh) (PK_id exp.sh.raw_sh) in
-  let both_honest = honest ip i in
+let composed_id (#oparams:odh_parameters) (sh1:share oparams) (sh2:share oparams{
+    sh1.raw_sh <> sh2.raw_sh
+  }) =
+  let le_sh1 = little_endian sh1.raw_sh in
+  let le_sh2 = little_endian sh2.raw_sh in
+  if le_sh1 < le_sh2 then
+    sh1.raw_sh,sh2.raw_sh
+  else
+    sh2.raw_sh,sh1.raw_sh
+
+let dh_op_memory_footprint
+  (#oparams:odh_parameters)
+  (#ip:odh_index_package oparams)
+  (#kp:key_package (composed_ip ip) oparams)
+  (op:odh_package ip kp)
+  (sh:share oparams)
+  (exp:exponent oparams{
+    exp.sh.raw_sh <> sh.raw_sh
+  })
+  (h0:mem)
+  (h1:mem) =
+  let i:id (composed_ip ip) = composed_id sh exp.sh in
+  let both_honest = honest i in
   ((both_honest /\ Flags.prf_odh) ==>
-    (match MM.sel (sel h0 op.kp_log) i with
+    (let log:i_key_log op.log_rgn (composed_ip ip) kp.key_type = op.log in
+    match MM.sel (sel h0 log) i with
     | Some _ ->
       modifies Set.empty h0 h1
     | None ->
-      modifies (Set.singleton op.kp_log_rgn) h0 h1))
+      modifies (Set.singleton op.log_rgn) h0 h1))
   /\ ((~both_honest \/ ~Flags.prf_odh) ==>
       modifies Set.empty h0 h1)
 
-let dh_op_log_change (#ip:index_package) (#key_length:(n:nat{n<=32})) (#key_type:(inst_id -> Type0)) (#kp:key_package ip key_length key_type) (#oparam:odh_parameters{oparam.hash_length = key_length}) (op:odh_package kp oparam) (sh:share oparam) (exp:exponent oparam{exp.sh.raw_sh <> sh.raw_sh}) (h0:mem) (h1:mem) =
-  let i = compose_id (PK_id sh.raw_sh) (PK_id exp.sh.raw_sh) in
-  let both_honest = honest ip i in
-  contains h0 op.kp_log
-  /\ ((both_honest /\ Flags.prf_odh) ==>
-      (MM.defined op.kp_log i h0 ==>
-        Some? (sel h1 op.kp_log i)
-        /\ (let k = Some?.v (sel h1 op.kp_log i) in
-          sel h1 op.kp_log == sel h0 op.kp_log
-        /\ witnessed (MM.contains op.kp_log i k)))
-      /\ (MM.fresh op.kp_log i h0 ==>
-          Some? (sel h1 op.kp_log i)
-          /\ (let k = Some?.v (sel h1 op.kp_log i) in
-          witnessed (MM.contains op.kp_log i k)
-          /\ sel h1 op.kp_log == MM.upd (sel h0 op.kp_log) i k))
-    )
-  /\ ((~both_honest \/ ~Flags.prf_odh) ==>
-      sel h1 op.kp_log == sel h0 op.kp_log)
+let dh_op_log_change
+  (#oparams:odh_parameters)
+  (#ip:odh_index_package oparams)
+  (#kp:key_package (composed_ip ip) oparams)
+  (op:odh_package ip kp)
+  (sh:share oparams)
+  (exp:exponent oparams{
+    exp.sh.raw_sh <> sh.raw_sh
+  })
+  (h0:mem)
+  (h1:mem) =
+  let i:id (composed_ip ip) = composed_id sh exp.sh in
+  let both_honest = honest i in
+  if Flags.model then
+    (let log:i_key_log op.log_rgn (composed_ip ip) kp.key_type = op.log in
+    contains h0 log
+    /\ ((both_honest /\ Flags.prf_odh) ==>
+        (MM.defined log i h0 ==>
+          Some? (sel h1 log i)
+          /\ (let k = Some?.v (sel h1 log i) in
+            sel h1 log == sel h0 log
+          /\ witnessed (MM.contains log i k)))
+        /\ (MM.fresh log i h0 ==>
+            Some? (sel h1 log i)
+            /\ (let k = Some?.v (sel h1 log i) in
+            witnessed (MM.contains log i k)
+            /\ sel h1 log == MM.upd (sel h0 log) i k))
+      ))
+  else
+    True
 
 // Do we need/want this?
-let dh_op_functional_spec (#ip:index_package) (#key_length:(n:nat{n<=32})) (#key_type:(inst_id -> Type0)) (#kp:key_package ip key_length key_type) (#oparam:odh_parameters{oparam.hash_length = key_length}) (op:odh_package kp oparam) (sh:share oparam) (exp:exponent oparam{exp.sh.raw_sh <> sh.raw_sh}) (k:key_type (compose_id (PK_id sh.raw_sh) (PK_id exp.sh.raw_sh))) (h1:mem) =
-  let i = compose_id (PK_id sh.raw_sh) (PK_id exp.sh.raw_sh) in
-  let both_honest = honest ip i in
+let dh_op_functional_spec
+  (#oparams:odh_parameters)
+  (#ip:odh_index_package oparams)
+  (#kp:key_package (composed_ip ip) oparams)
+  (op:odh_package ip kp)
+  (sh:share oparams)
+  (exp:exponent oparams{
+    exp.sh.raw_sh <> sh.raw_sh
+  })
+  (k:kp.key_type (composed_id sh exp.sh))
+  (h1:mem) =
+  let i:id (composed_ip ip) = composed_id sh exp.sh in
+  let both_honest = honest i in
     ((Flags.prf_odh /\ both_honest) ==>
-        (Some? (MM.sel (sel h1 op.kp_log) i)
-        /\ k == Some?.v (MM.sel (sel h1 op.kp_log) i)
-        /\ honest ip i
+        (let log:i_key_log op.log_rgn (composed_ip ip) kp.key_type = op.log in
+        Some? (MM.sel (sel h1 log) i)
+        /\ k == Some?.v (MM.sel (sel h1 log) i)
+        /\ honest i
       )) // If possible, indicate somehow that k was randomly drawn.
     /\ (~Flags.prf_odh ==>
-        kp.getGT k == oparam.hash (oparam.exponentiate exp.raw_exp sh.raw_sh)
-        /\ (both_honest ==> honest ip i)
-        /\ ~both_honest ==> dishonest ip i)
+        kp.getGT k == oparams.hash (oparams.exponentiate exp.raw_exp sh.raw_sh)
+        /\ (both_honest ==> honest i)
+        /\ ~both_honest ==> corrupt i)
 
-
-#set-options "--z3rlimit 300 --max_ifuel 2 --max_fuel 1"
-val dh_op: (#ip:index_package) ->  (#key_length:(n:nat{n<=32})) -> (#key_type:(inst_id -> Type0)) -> (#kp:key_package ip key_length key_type) -> (#oparam:odh_parameters{oparam.hash_length = key_length}) -> op:odh_package kp oparam -> sh:share oparam -> exp:exponent oparam{exp.sh.raw_sh <> sh.raw_sh} -> ST (key_type (compose_id (PK_id sh.raw_sh) (PK_id exp.sh.raw_sh)))
-  (requires (fun h0 ->
-    let i = compose_id (PK_id sh.raw_sh) (PK_id exp.sh.raw_sh) in
-    (kp.flag ==> Flags.prf_odh)
-    /\ registered ip i
-  ))
-  (ensures (fun h0 k h1 ->
-    let i = compose_id (PK_id sh.raw_sh) (PK_id exp.sh.raw_sh) in
-    let both_honest = honest ip i in
-    dh_op_memory_footprint op sh exp h0 h1
-    /\ dh_op_log_change op sh exp h0 h1
-    /\ dh_op_functional_spec op sh exp k h1
-  ))
+#set-options "--z3rlimit 50 --max_ifuel 2 --max_fuel 2"
+val dh_op:
+  (#oparams:odh_parameters) ->
+  (#ip:odh_index_package oparams) ->
+  (#kp:key_package (composed_ip ip) oparams) ->
+  (op:odh_package ip kp) ->
+  (sh:share oparams) ->
+  (exp:exponent oparams{exp.sh.raw_sh <> sh.raw_sh}) ->
+  ST (kp.key_type (composed_id sh exp.sh))
+    (requires (fun h0 ->
+      let i:id (composed_ip ip) = composed_id sh exp.sh in
+      (kp.flag ==> Flags.prf_odh)
+      /\ registered #(composed_ip ip) i
+    ))
+    (ensures (fun h0 k h1 ->
+      let i:id (composed_ip ip) = composed_id sh exp.sh in
+      let both_honest = honest #(composed_ip ip) i in
+      dh_op_memory_footprint op sh exp h0 h1
+      /\ dh_op_log_change op sh exp h0 h1
+      /\ dh_op_functional_spec op sh exp k h1
+    ))
