secure_api/box/Box.PKAE.fst
@@ -14,6 +14,7 @@ module ODH = Box.ODH
 module MM = FStar.Monotonic.Map
 module AE_Spec = Spec.SecretBox
 module ODH_Spec = Spec.Curve25519
+module PKAE_Spec = Spec.CryptoBox
 module H = Spec.HSalsa20
 
 assume val random_bytes: n:nat -> lbytes n
@@ -23,13 +24,17 @@ assume val random_bytes: n:nat -> lbytes n
 val ae_enc_star: n:(n:nat{AE_Spec.valid_plain_length n}) -> b:lbytes (n+16){AE_Spec.valid_cipher_length (n+16)}
 let ae_enc_star n = Seq.append (random_bytes n) (random_bytes 16)
 
+let pp = PP Flags.pkae AE_Spec.valid_plain_length AE_Spec.valid_cipher_length (fun n -> n = AE_Spec.noncelen)
+
 // For some reason it doesn't verify if there is an additional refinement on the output of secretbox_open_easy
+#set-options "--z3rlimit 300 --max_ifuel 1 --max_fuel 0"
 let secretbox_scheme =
-  AE.ES #(AE_Spec.keylen) #(AE_Spec.noncelen) (AE_Spec.valid_plain_length) (AE_Spec.valid_cipher_length) (fun () -> random_bytes 32) AE_Spec.secretbox_easy (ae_enc_star) AE_Spec.secretbox_open_easy
+  let ss = AE.ES #(AE_Spec.keylen) #pp (fun () -> random_bytes 32) AE_Spec.secretbox_easy (ae_enc_star) AE_Spec.secretbox_open_easy in
+  ss
 
-let ae_params = AE.GP AE_Spec.keylen AE_Spec.noncelen secretbox_scheme
-
-
+let ae_params =
+  let aep = AE.GP AE_Spec.keylen secretbox_scheme in
+  aep
 
 //let ae_package_log_key = i:ODH.id
 //let ae_package_log_value (rgn:erid) (i:ODH.id) = (ap:AE.ae_package #ODH.id #i #AE_Spec.keylen kp ae_params pp{extends (AE.get_ap_rgn ap) rgn})
@@ -44,26 +49,24 @@ let hsalsa20_hash input = H.hsalsa20 input zero_nonce
 
 let odh_params = ODH.OP (ODH_Spec.serialized_point_length) (ODH_Spec.scalar_length) (H.keylen) (ODH_Spec.base_point) (ODH_Spec.scalarmult) (hsalsa20_hash)
 
-#set-options "--z3rlimit 30 --max_ifuel 1 --max_fuel 0"
-noeq abstract type pkae_package =
+#set-options "--z3rlimit 300 --max_ifuel 1 --max_fuel 0"
+noeq abstract type pkae_package (#pp:plain_package) (#pkp:pkae_parameters pp) (ip:index_package pkp) =
   | PKAE_P :
     pkae_rgn:erid ->
-    ip: index_package ->
-    pp: plain_package{pp.flag == Flags.pkae /\ pp.valid_length == AE_Spec.valid_plain_length} ->
     kp: Key.key_package ip AE_Spec.keylen (AE.key AE_Spec.keylen) ->
     op: ODH.odh_package #ip #AE_Spec.keylen #(AE.key AE_Spec.keylen) kp odh_params ->
-    ap: AE.ae_package kp ae_params{AE.get_ap_pp ap == pp} ->
+    ap: AE.ae_package kp ae_params ->
     pkae_package
 
-#set-options "--z3rlimit 30 --max_ifuel 1 --max_fuel 0"
-let create_pkae_package rgn =
+#set-options "--z3rlimit 300 --max_ifuel 1 --max_fuel 0"
+let create_pkae_package rgn pp =
   let pkae_rgn = new_region rgn in
   let ip = create_index_package pkae_rgn in
-  let pp = PP Flags.pkae AE_Spec.valid_plain_length in
+  //let pp = PP Flags.pkae AE_Spec.valid_plain_length in
   let kp = AE.create_ae_key_package ip AE_Spec.keylen in
   let op = ODH.create_odh_package pkae_rgn kp odh_params in
   let ap = AE.create_ae_package pkae_rgn kp ae_params in
-  PKAE_P pkae_rgn ip pp kp op ap
+  PKAE_P pkae_rgn ip kp op ap
 
 let pkey = ODH.share odh_params
 let get_pkey_raw = ODH.get_share_raw
@@ -78,32 +81,27 @@ let get_skey_id sk = get_pkey_id (ODH.get_exp_share sk)
 //let nonce = AE.nonce ae_params
 //let ciphertext = AE.ciphertext ae_params
 
-let get_index_package pkae_p = pkae_p.ip
+let get_index_package #pp pkae_p = pkae_p.ip
 
-let gen_footprint pkae_p h0 h1 = ODH.gen_dh_footprint pkae_p.ip odh_params h0 h1
+let gen_footprint #pp pkae_p h0 h1 = ODH.gen_dh_footprint pkae_p.ip odh_params h0 h1
 
-let gen pkae_p = ODH.gen_dh pkae_p.ip odh_params
+let gen #pp pkae_p = ODH.gen_dh pkae_p.ip odh_params
 
-let coerce_pkey_footprint pkae_p pk_raw h0 h1 = ODH.coerce_dh_sh_footprint pkae_p.ip odh_params pk_raw h0 h1
+let coerce_pkey_footprint #pp pkae_p pk_raw h0 h1 = ODH.coerce_dh_sh_footprint pkae_p.ip odh_params pk_raw h0 h1
 
-let coerce_pkey pkae_p pk_raw =
+let coerce_pkey #pp pkae_p pk_raw =
   let pk = ODH.coerce_dh_sh pkae_p.ip odh_params pk_raw in
   pk
 
-let coerce_skey_footprint pkae_p sk_raw h0 h1 = ODH.coerce_dh_exp_footprint pkae_p.ip odh_params sk_raw h0 h1
+let coerce_skey_footprint #pp pkae_p sk_raw h0 h1 = ODH.coerce_dh_exp_footprint pkae_p.ip odh_params sk_raw h0 h1
 
-let coerce_skey pkae_p sk_raw =
+let coerce_skey #pp pkae_p sk_raw =
   let sk = ODH.coerce_dh_exp pkae_p.ip odh_params sk_raw in
   sk
 
 let compose_ids pk1 pk2 = compose_id (pk1) pk2
 
-let nonce = AE.nonce ae_params
-let ciphertext = AE.ciphertext ae_params
-
-let valid_ciphertext_length = AE_Spec.valid_cipher_length
-
-let compatible_keys pk sk = get_pkey_from_skey sk <> pk
+//let compatible_keys pk sk = get_pkey_from_skey sk <> pk
 
 //#set-options "--z3rlimit 5 --max_ifuel 0 --max_fuel 0"
 //val create_key : pkae_p:pkae_package -> i:inst_id -> message_log_value i
@@ -115,197 +113,177 @@ let compatible_keys pk sk = get_pkey_from_skey sk <> pk
 //  //let pkae_value : message_log_value i = ae_value in
 //  //pkae_value
 
-let get_log_rgn pkae_p = AE.get_log_rgn pkae_p.ap
+let get_log_rgn #pp pkae_p = AE.get_log_rgn pkae_p.ap
 
-let get_pp pkae_p = AE.get_ap_pp pkae_p.ap
+// We need an explicit ciphertext type with valid_length predicate.
+//val get_pp: pkae_p:pkae_package -> pp:plain_package{pp.flag == Flags.pkae /\ pp.valid_length}
+//let get_pp #pp pkae_p = AE.get_ap_pp pkae_p.ap
 
-#set-options "--z3rlimit 100 --max_ifuel 2 --max_fuel 0"
+#set-options "--z3rlimit 300 --max_ifuel 1 --max_fuel 0"
 //val get_log: pkae_p:pkae_package -> GTot (AE.ae_message_log ae_params (AE.get_ap_pp pkae_p.ap) (AE.get_log_rgn pkae_p.ap))
 //val get_log: pkae_p:pkae_package -> GTot (AE.ae_message_log ae_params (AE.get_ap_pp pkae_p.ap) (AE.get_log_rgn pkae_p.ap))
-let get_log pkae_p =
-  AE.get_ap_log pkae_p.ap
+let get_log #pp pkae_p =
+  assert(ae_params.AE.scheme.AE.pp == pp);
+  admit()
+  //AE.get_ap_log #pkae_p.ip #_ #_ #ae_params pkae_p.ap
 
+let encrypt_footprint pkae_p pk sk n c p h0 h1 =
+  ODH.dh_op_memory_footprint pkae_p.op pk sk h0 h1
+  /\ AE.encrypt_footprint pkae_p.ap h0 h1
 
-//#set-options "--z3rlimit 300 --max_ifuel 0 --max_fuel 0"
-//val get_ap_from_log: pkae_p:pkae_package -> i:ODH.id -> ST (option (ap:ae_package_log_value pkae_p.ap_rgn i))
-//  (requires (fun h0 -> True))
-//  (ensures (fun h0 ap h1 ->
-//    (match sel h0 pkae_p.ap_log i with
-//      | Some ap ->
-//        contains h1 (AE.get_ap_log ap)
-//        /\ MM.defined pkae_p.ap_log i h1
-//        /\ MM.contains pkae_p.ap_log i ap h1
-//        /\ witnessed (MM.defined pkae_p.ap_log i)
-//        /\ witnessed (MM.contains pkae_p.ap_log i ap)
-//      | None -> MM.fresh pkae_p.ap_log i h1)
-//    /\ h0 == h1
-//    /\ ap == MM.sel (sel h1 pkae_p.ap_log) i
-//  ))
-//
-//let get_ap_from_log pkae_p i =
-//  match MM.lookup pkae_p.ap_log i with
-//  | Some ap ->
-//    AE.recall_log ap;
-//    Some ap
-//  | None -> None
-//
-//
-////#set-options "--z3rlimit 300 --max_ifuel 0 --max_fuel 0"
-////val nonce_freshness_framing_lemma: pkae_p:pkae_package -> i:ODH.id -> n:nonce -> h0:mem -> h1:mem -> Lemma
-////  (requires (
-////    //((modifies (Set.singleton (ODH.get_op_rgn pkae_p.op)) h0 h1 /\ (extends (ODH.get_op_rgn pkae_p.op) pkae_p.op_rgn)) \/ h0 == h1)
-////    (modifies (Set.singleton (ODH.get_op_rgn pkae_p.op)) h0 h1 \/ h0 == h1)
-////    /\ extends (ODH.get_op_rgn pkae_p.op) pkae_p.op_rgn
-////    /\ disjoint (ODH.get_op_rgn pkae_p.op) pkae_p.ap_log_rgn
-////    /\ contains h0 pkae_p.ap_log
-////    /\ (match sel h0 pkae_p.ap_log i with
-////      | Some ap -> contains h0 (AE.get_ap_log ap)
-////      | None -> True)
-////  ))
-////  (ensures (
-////    contains h1 pkae_p.ap_log
-////    /\ (match sel h0 pkae_p.ap_log i with
-////      | Some ap_old ->
-////        let ap_new = Some?.v (sel h1 pkae_p.ap_log i) in
-////        AE.get_ap_log ap_old == AE.get_ap_log ap_new
-////        /\ contains h1 (AE.get_ap_log ap_new)
-////      | None -> True)
-////    ///\ (let ap_option_new = sel h1 pkae_p.ap_log i in
-////    //ap_option_new == ap_option_old
-////    ///\ (Some? ap_option_new)
-////    ///\ AE.get_ap_log (Some?.v ap_option_new) == AE.get_ap_log (Some?.v ap_option_old))
-////  ))
-////let nonce_freshness_framing_lemma pkae_p i n h0 h1 = ()
-//
-//#set-options "--z3rlimit 300 --max_ifuel 0 --max_fuel 0"
-//val encrypt: pkae_package:pkae_package -> pk:pkey -> sk:skey{ODH.get_share_raw pk <> ODH.get_share_raw (ODH.get_exp_share sk)} -> n:nonce -> p:protected_plain pp (ODH.create_id pk (ODH.get_exp_share sk)) -> ST ciphertext
-//  (requires (fun h0 ->
-//    let i = ODH.create_id pk (ODH.get_exp_share sk) in
-//    match sel h0 pkae_package.ap_log i with
-//    | Some ap ->
-//      contains h0 (AE.get_ap_log ap)
-//      /\ AE.nonce_is_unique ap n h0
-//    | None -> True
-//  ))
-//  (ensures (fun h0 c h1 ->
-//    let i = ODH.create_id pk (ODH.get_exp_share sk) in
-//    let both_honest = ODH.exp_hon sk && ODH.sh_hon pk in
-//    let kp_log = ODH.get_op_log pkae_package.op in
-//    // Describe ap_log state
-//    Some? (sel h1 pkae_package.ap_log i)
-//    /\ (let ap = Some?.v (sel h1 pkae_package.ap_log i) in
-//    (if Some? (sel h0 pkae_package.ap_log i) then
-//      sel h1 pkae_package.ap_log == sel h0 pkae_package.ap_log
-//      /\ sel h1 (AE.get_ap_log ap) == MM.upd (sel h0 (AE.get_ap_log ap)) (n,c) p
-//    else
-//      sel h1 pkae_package.ap_log == MM.upd (sel h0 pkae_package.ap_log) i ap
-//      /\ (forall n' . n' =!= n ==> AE.nonce_is_unique ap n' h1))
-//    // Describe modified memory regions
-//    /\ (let modified_regions_ap_op = Set.union
-//        (AE.encrypt_modified_regions ap)
-//        (ODH.dh_op_modified_regions pkae_package.op pk sk h0)
-//      in
-//      let modified_regions_extend_ap_log = Set.union (Set.singleton pkae_package.ap_rgn) (Set.singleton pkae_package.ap_log_rgn) in
-//      let modified_regions =
-//        if Some? (sel h0 pkae_package.ap_log i) then
-//          modified_regions_ap_op
-//        else
-//          Set.union modified_regions_ap_op modified_regions_extend_ap_log
-//      in
-//      modifies modified_regions h0 h1)
-//    /\ ODH.dh_op_log_change pkae_package.op pk sk h0 h1
-//    // Describe functionality
-//    /\ (let k =
-//        if both_honest && ODH.get_flag() then
-//          Some?.v (MM.sel (sel h1 (ODH.get_op_log pkae_package.op)) i)
-//        else
-//          ODH.(odh_params.hash (odh_params.exponentiate (ODH.get_exponent_raw sk) (ODH.get_share_raw pk)))
-//      in
-//      ODH.dh_op_functional_spec pkae_package.op pk sk k h1
-//    )
-//    /\ ((both_honest /\ ODH.get_flag()) ==>
-//        (let k = Some?.v (MM.sel (sel h1 (ODH.get_op_log pkae_package.op)) i) in
-//        AE.encrypt_functional_spec ap k n c p)
-//      )
-//      // In case we have a dishonest key or we don't idealize, we can't guarantee anything.
-//    )
-//  ))
-//
-//#set-options "--z3rlimit 300 --max_ifuel 0 --max_fuel 0"
-//let encrypt pkae_package pk sk n p =
-//  let i = ODH.create_id pk (ODH.get_exp_share sk) in
-//  recall pkae_package.ap_log;
-//  let k = ODH.dh_op pkae_package.op pk sk in
-//  let h1 = get() in
-//  ODH.recall_op_log pkae_package.op;
-//  let ap =
-//    match get_ap_from_log pkae_package i with
-//    | Some ap ->
-//      ap
-//    | None ->
-//      let ap = AE.create_ae_package pkae_package.ap_rgn kp ae_params pp in
-//      MM.extend pkae_package.ap_log i ap;
-//      ap
-//  in
-//  let c = AE.encrypt ap k n p in
-//  //assert(
-//  //    let both_honest = ODH.exp_hon sk && ODH.sh_hon pk in
-//  //    (both_honest /\ ODH.get_flag()) ==>
-//  //      (let k' = Some?.v (MM.sel (sel h1 (ODH.get_op_log pkae_package.op)) i) in
-//  //      AE.encrypt_functional_spec ap k n c p
-//  //      )
-//  //    );
-//  //    admit();
-//  //assert(AE.encrypt_functional_spec ap k n c p);
-//  c
-//
-//val decrypt: pkae_package:pkae_package -> pk:pkey -> sk:skey{ODH.get_share_raw pk <> ODH.get_share_raw (ODH.get_exp_share sk)} -> n:nonce -> c:ciphertext -> ST (option (p:protected_plain pp (ODH.create_id pk (ODH.get_exp_share sk))))
-//  (requires (fun h0 ->
-//    let i = ODH.create_id pk (ODH.get_exp_share sk) in
-//    match sel h0 pkae_package.ap_log i with
-//    | Some ap ->
-//      contains h0 (AE.get_ap_log ap)
-//    | None -> True
-//  ))
-//  (ensures (fun h0 c h1 ->
-//    let i = ODH.create_id pk (ODH.get_exp_share sk) in
-//    let both_honest = ODH.exp_hon sk && ODH.sh_hon pk in
-//    let kp_log = ODH.get_op_log pkae_package.op in
-//    match sel h0 pkae_package.ap_log i with
-//    | Some ap ->
-//      ((both_honest /\ ODH.get_flag()) ==>
-//        (MM.defined kp_log i h0 ==>
-//          h0 == h1)
-//        /\ (MM.fresh kp_log i h0 ==>
-//          modifies (Set.singleton (ODH.get_op_rgn pkae_package.op)) h0 h1))
-//      /\ ((~both_honest \/ ~(ODH.get_flag())) ==>
-//          h0 == h1)
-//    | None ->
-//      MM.defined pkae_package.ap_log i h1
-//      /\ (let ap = Some?.v (sel h1 pkae_package.ap_log i) in
-//        sel h1 pkae_package.ap_log == MM.upd (sel h0 pkae_package.ap_log) i ap
-//        /\ ((both_honest /\ ODH.get_flag()) ==>
-//            (MM.defined kp_log i h0 ==>
-//              modifies (Set.union (Set.singleton pkae_package.ap_rgn) (Set.singleton pkae_package.ap_log_rgn)) h0 h1)
-//            /\ (MM.fresh kp_log i h0 ==>
-//              modifies (Set.union (Set.singleton pkae_package.ap_rgn) (Set.union (Set.singleton pkae_package.ap_log_rgn) (Set.singleton (ODH.get_op_rgn pkae_package.op)))) h0 h1))
-//        /\ ((~both_honest \/ ~(ODH.get_flag())) ==>
-//            (modifies (Set.union (Set.singleton pkae_package.ap_rgn) (Set.singleton pkae_package.ap_log_rgn)) h0 h1)))
-//  ))
-//
-//let decrypt pkae_package pk sk n c =
-//  let i = ODH.create_id pk (ODH.get_exp_share sk) in
-//  recall pkae_package.ap_log;
-//  let k = ODH.dh_op pkae_package.op pk sk in
-//  let ap =
-//    match get_ap_from_log pkae_package i with
-//    | Some ap ->
-//      ap
-//    | None ->
-//      let ap = AE.create_ae_package pkae_package.ap_rgn kp ae_params pp in
-//      MM.extend pkae_package.ap_log i ap;
-//      recall pkae_package.ap_log;
-//      AE.recall_log ap;
-//      ap
-//  in
-//  AE.decrypt ap k n c
+let decrypt_footprint pkae_p pk sk n c p h0 h1 =
+  ODH.dh_op_memory_footprint pkae_p.op pk sk h0 h1
+  /\ AE.decrypt_footprint pkae_p.ap h0 h1
+
+let enc_spec pkae_p p pk sk n = PKAE_Spec.cryptobox p n pk sk
+
+// Maybe require function to get cipher length from plain_length
+let enc_star pkae_p plain_length = random_bytes (plain_length+16)
+
+val dec_spec: pkae_p:pkae_package -> c:ciphertext -> pk:lbytes pkey_length -> sk:lbytes skey_length -> n:nonce -> option (p:plain (get_pp pkae_p))
+
+#set-options "--z3rlimit 100 --max_ifuel 1 --max_fuel 0"
+let dec_spec pkae_p c pk sk n =
+  let option_p:option (plain pkae_p.pp) = PKAE_Spec.cryptobox_open c n pk sk in
+  assert(pkae_p.pp == get_pp pkae_p);
+  match option_p with
+  | Some (p:plain (pkae_p.pp)) ->
+    let (p:plain (get_pp pkae_p)) = p in
+    admit()
+    //Some p
+  | None -> None
+  //let option_pp:option (plain (get_pp pkae_p)) = option_p in
+  //admit()
+
+#set-options "--z3rlimit 300 --max_ifuel 0 --max_fuel 0"
+val encrypt: pkae_package:pkae_package -> pk:pkey -> sk:skey{ODH.get_share_raw pk <> ODH.get_share_raw (ODH.get_exp_share sk)} -> n:nonce -> p:protected_plain pp (ODH.create_id pk (ODH.get_exp_share sk)) -> ST ciphertext
+  (requires (fun h0 ->
+    let i = ODH.create_id pk (ODH.get_exp_share sk) in
+    match sel h0 pkae_package.ap_log i with
+    | Some ap ->
+      contains h0 (AE.get_ap_log ap)
+      /\ AE.nonce_is_unique ap n h0
+    | None -> True
+  ))
+  (ensures (fun h0 c h1 ->
+    let i = ODH.create_id pk (ODH.get_exp_share sk) in
+    let both_honest = ODH.exp_hon sk && ODH.sh_hon pk in
+    let kp_log = ODH.get_op_log pkae_package.op in
+    // Describe ap_log state
+    Some? (sel h1 pkae_package.ap_log i)
+    /\ (let ap = Some?.v (sel h1 pkae_package.ap_log i) in
+    (if Some? (sel h0 pkae_package.ap_log i) then
+      sel h1 pkae_package.ap_log == sel h0 pkae_package.ap_log
+      /\ sel h1 (AE.get_ap_log ap) == MM.upd (sel h0 (AE.get_ap_log ap)) (n,c) p
+    else
+      sel h1 pkae_package.ap_log == MM.upd (sel h0 pkae_package.ap_log) i ap
+      /\ (forall n' . n' =!= n ==> AE.nonce_is_unique ap n' h1))
+    // Describe modified memory regions
+    /\ (let modified_regions_ap_op = Set.union
+        (AE.encrypt_modified_regions ap)
+        (ODH.dh_op_modified_regions pkae_package.op pk sk h0)
+      in
+      let modified_regions_extend_ap_log = Set.union (Set.singleton pkae_package.ap_rgn) (Set.singleton pkae_package.ap_log_rgn) in
+      let modified_regions =
+        if Some? (sel h0 pkae_package.ap_log i) then
+          modified_regions_ap_op
+        else
+          Set.union modified_regions_ap_op modified_regions_extend_ap_log
+      in
+      modifies modified_regions h0 h1)
+    /\ ODH.dh_op_log_change pkae_package.op pk sk h0 h1
+    // Describe functionality
+    /\ (let k =
+        if both_honest && ODH.get_flag() then
+          Some?.v (MM.sel (sel h1 (ODH.get_op_log pkae_package.op)) i)
+        else
+          ODH.(odh_params.hash (odh_params.exponentiate (ODH.get_exponent_raw sk) (ODH.get_share_raw pk)))
+      in
+      ODH.dh_op_functional_spec pkae_package.op pk sk k h1
+    )
+    /\ ((both_honest /\ ODH.get_flag()) ==>
+        (let k = Some?.v (MM.sel (sel h1 (ODH.get_op_log pkae_package.op)) i) in
+        AE.encrypt_functional_spec ap k n c p)
+      )
+      // In case we have a dishonest key or we don't idealize, we can't guarantee anything.
+    )
+  ))
+
+#set-options "--z3rlimit 300 --max_ifuel 0 --max_fuel 0"
+let encrypt pkae_package pk sk n p =
+  let i = ODH.create_id pk (ODH.get_exp_share sk) in
+  recall pkae_package.ap_log;
+  let k = ODH.dh_op pkae_package.op pk sk in
+  let h1 = get() in
+  ODH.recall_op_log pkae_package.op;
+  let ap =
+    match get_ap_from_log pkae_package i with
+    | Some ap ->
+      ap
+    | None ->
+      let ap = AE.create_ae_package pkae_package.ap_rgn kp ae_params pp in
+      MM.extend pkae_package.ap_log i ap;
+      ap
+  in
+  let c = AE.encrypt ap k n p in
+  //assert(
+  //    let both_honest = ODH.exp_hon sk && ODH.sh_hon pk in
+  //    (both_honest /\ ODH.get_flag()) ==>
+  //      (let k' = Some?.v (MM.sel (sel h1 (ODH.get_op_log pkae_package.op)) i) in
+  //      AE.encrypt_functional_spec ap k n c p
+  //      )
+  //    );
+  //    admit();
+  //assert(AE.encrypt_functional_spec ap k n c p);
+  c
+
+val decrypt: pkae_package:pkae_package -> pk:pkey -> sk:skey{ODH.get_share_raw pk <> ODH.get_share_raw (ODH.get_exp_share sk)} -> n:nonce -> c:ciphertext -> ST (option (p:protected_plain pp (ODH.create_id pk (ODH.get_exp_share sk))))
+  (requires (fun h0 ->
+    let i = ODH.create_id pk (ODH.get_exp_share sk) in
+    match sel h0 pkae_package.ap_log i with
+    | Some ap ->
+      contains h0 (AE.get_ap_log ap)
+    | None -> True
+  ))
+  (ensures (fun h0 c h1 ->
+    let i = ODH.create_id pk (ODH.get_exp_share sk) in
+    let both_honest = ODH.exp_hon sk && ODH.sh_hon pk in
+    let kp_log = ODH.get_op_log pkae_package.op in
+    match sel h0 pkae_package.ap_log i with
+    | Some ap ->
+      ((both_honest /\ ODH.get_flag()) ==>
+        (MM.defined kp_log i h0 ==>
+          h0 == h1)
+        /\ (MM.fresh kp_log i h0 ==>
+          modifies (Set.singleton (ODH.get_op_rgn pkae_package.op)) h0 h1))
+      /\ ((~both_honest \/ ~(ODH.get_flag())) ==>
+          h0 == h1)
+    | None ->
+      MM.defined pkae_package.ap_log i h1
+      /\ (let ap = Some?.v (sel h1 pkae_package.ap_log i) in
+        sel h1 pkae_package.ap_log == MM.upd (sel h0 pkae_package.ap_log) i ap
+        /\ ((both_honest /\ ODH.get_flag()) ==>
+            (MM.defined kp_log i h0 ==>
+              modifies (Set.union (Set.singleton pkae_package.ap_rgn) (Set.singleton pkae_package.ap_log_rgn)) h0 h1)
+            /\ (MM.fresh kp_log i h0 ==>
+              modifies (Set.union (Set.singleton pkae_package.ap_rgn) (Set.union (Set.singleton pkae_package.ap_log_rgn) (Set.singleton (ODH.get_op_rgn pkae_package.op)))) h0 h1))
+        /\ ((~both_honest \/ ~(ODH.get_flag())) ==>
+            (modifies (Set.union (Set.singleton pkae_package.ap_rgn) (Set.singleton pkae_package.ap_log_rgn)) h0 h1)))
+  ))
+
+let decrypt pkae_package pk sk n c =
+  let i = ODH.create_id pk (ODH.get_exp_share sk) in
+  recall pkae_package.ap_log;
+  let k = ODH.dh_op pkae_package.op pk sk in
+  let ap =
+    match get_ap_from_log pkae_package i with
+    | Some ap ->
+      ap
+    | None ->
+      let ap = AE.create_ae_package pkae_package.ap_rgn kp ae_params pp in
+      MM.extend pkae_package.ap_log i ap;
+      recall pkae_package.ap_log;
+      AE.recall_log ap;
+      ap
+  in
+  AE.decrypt ap k n c
