secure_api/box/Mem.fst
@@ -8,17 +8,25 @@ open Box.Plain
 
 
 module MM = FStar.Monotonic.Map
+module Flags = Box.Flags
 
-type message_log_key (nonce:Type0) (ciphertext:Type0) = inst_id*nonce*ciphertext
-//  | LOG_KEY: i:inst_id -> n:nonce aparams -> c:ciphertext aparams -> message_log_key aparams
+// Merge this file with plain?
 
-let message_log_value (pp:plain_package) (i:inst_id) = protected_plain pp i
-let message_log_range (#nonce:Type0) (#ciphertext:Type0) (pp:plain_package)  (k:message_log_key nonce ciphertext) = message_log_value pp (Mktuple3?._1 k)
-let message_log_inv (#nonce:Type0) (#ciphertext:Type0) (#pp:plain_package) (f:MM.map' (message_log_key nonce ciphertext) (message_log_range pp)) = True
+type message_log_key (ip:index_package) (pp:plain_package) = id ip*nonce pp*cipher pp
+//  | LOG_KEY: i:id ip -> n:nonce aparams -> c:ciphertext aparams -> message_log_key aparams
 
-let message_log (nonce:Type0) (ciphertext:Type0) (pp:plain_package) (rgn:erid) =
-  MM.t rgn (message_log_key nonce ciphertext) (message_log_range pp) (message_log_inv)
+let message_log_value (#ip:index_package) (pp:plain_package) (i:id ip) = protected_plain pp i
+let message_log_range (#ip:index_package)(pp:plain_package)  (k:message_log_key ip pp) = message_log_value pp (Mktuple3?._1 k)
+let message_log_inv (#ip:index_package) (#pp:plain_package) (f:MM.map' (message_log_key ip pp) (message_log_range pp)) = True
 
-let empty_message_log (nonce:Type0) (ciphertext:Type0) (pp:plain_package) = MM.empty_map (message_log_key nonce ciphertext) (message_log_range pp)
+let i_message_log (ip:index_package) (pp:plain_package) (rgn:erid) =
+  MM.t rgn (message_log_key ip pp) (message_log_range pp) (message_log_inv)
+let message_log (ip:index_package) (pp:plain_package) (rgn:erid) =
+  if Flags.model then
+    MM.t rgn (message_log_key ip pp) (message_log_range pp) (message_log_inv)
+  else
+   unit
 
-let alloc_message_log (nonce:Type0) (ciphertext:Type0) (rgn:erid) (pp:plain_package) = MM.alloc #rgn #(message_log_key nonce ciphertext) #(message_log_range pp) #(message_log_inv)
+let empty_message_log (ip:index_package) (pp:plain_package) = MM.empty_map (message_log_key ip pp) (message_log_range pp)
+
+let alloc_message_log (rgn:erid) (ip:index_package) (pp:plain_package) = MM.alloc #rgn #(message_log_key ip pp) #(message_log_range pp) #(message_log_inv)
